Update to Lean v4.14.0-rc2

ReactorModel/Execution/Reactor.lean
@@ -7,7 +7,7 @@ namespace Reactor
 
 variable [Hierarchical α] in section
 
-def dependencies (rtr : α) (rcn : ID) : Set ID := 
+def dependencies (rtr : α) (rcn : ID) : Set ID :=
   { rcn' | rcn' <[rtr] rcn }
 
 structure Refresh (rtr₁ rtr₂ : α) (acts : ID ⇀ Value) : Prop where
@@ -22,8 +22,8 @@ end
 variable [Proper α] [Finite α]
 
 def refresh (rtr : α) (acts : ID ⇀ Value) : α :=
-  let rtr₁ := set rtr  .inp $ Partial.const (rtr[.inp].ids : Set ID) .absent
-  let rtr₂ := set rtr₁ .out $ Partial.const (rtr[.out].ids : Set ID) .absent
+  let rtr₁ := set rtr  .inp <| Partial.const (rtr[.inp].ids : Set ID) .absent
+  let rtr₂ := set rtr₁ .out <| Partial.const (rtr[.out].ids : Set ID) .absent
   set rtr₂ .act acts
 
 end Reactor
