ReactorModel/Execution/State.lean
@@ -1,7 +1,8 @@
+import Mathlib.Data.Finset.Max
 import ReactorModel.Execution.Reactor
 
 noncomputable section
-open Classical Reactor 
+open Classical Reactor
 
 namespace Execution
 
@@ -9,7 +10,7 @@ variable [Hierarchical α]
 
 @[ext]
 structure State (α) where
-  rtr      : α 
+  rtr      : α
   tag      : Time.Tag
   progress : Set ID
   events   : ID ⇀ Time.Tag ⇉ Value
@@ -19,47 +20,47 @@ namespace State
 def input (s : State α) (rcn : ID) : Reaction.Input where
   val cpt := s.rtr[.rcn][rcn] |>.elim ∅ (restriction · cpt)
   tag := s.tag
-where 
-  restriction (rcn : Reaction) (cpt : Component.Valued) := 
+where
+  restriction (rcn : Reaction) (cpt : Component.Valued) :=
     s.rtr[cpt].restrict { i | ⟨cpt, i⟩ ∈ rcn.deps .in }
 
-def output (s : State α) (rcn : ID) : Reaction.Output := 
-  s.rtr[.rcn][rcn] |>.elim [] (· $ s.input rcn)
+def output (s : State α) (rcn : ID) : Reaction.Output :=
+  s.rtr[.rcn][rcn] |>.elim [] (· <| s.input rcn)
 
-def record (s : State α) (rcn : ID) : State α := 
+def record (s : State α) (rcn : ID) : State α :=
   { s with progress := s.progress.insert rcn }
 
-def schedule (s : State α) (i : ID) (t : Time) (v : Value) : State α := 
+def schedule (s : State α) (i : ID) (t : Time) (v : Value) : State α :=
   { s with events := s.events.update i (go · t v) }
-where 
+where
   go (a : Time.Tag ⇉ Value) (t : Time) (v : Value) : Time.Tag ⇉ Value :=
     match a.keys.filter (·.time = t) |>.max with
     | ⊥           => a.insert ⟨t, 0⟩ v
     | some ⟨_, m⟩ => a.insert ⟨t, m + 1⟩ v
 
-def scheduledTags (s : State α) : Set Time.Tag := 
+def scheduledTags (s : State α) : Set Time.Tag :=
   { g | ∃ i a, (s.events i = some a) ∧ (g ∈ a.keys) }
 
-def actions (s : State α) (g : Time.Tag) : ID ⇀ Value := 
+def actions (s : State α) (g : Time.Tag) : ID ⇀ Value :=
   s.rtr[.act].mapIdx fun i => s.events i >>= (· g) |>.getD .absent
 
 def unprocessed (s : State α) : Set ID :=
   { i ∈ s.rtr[.rcn] | i ∉ s.progress }
 
 structure Allows (s : State α) (rcn : ID) : Prop where
-  mem         : rcn ∈ s.rtr[.rcn] 
+  mem         : rcn ∈ s.rtr[.rcn]
   deps        : dependencies s.rtr rcn ⊆ s.progress
   unprocessed : rcn ∉ s.progress
 
 inductive Triggers (s : State α) (i : ID) : Prop
-  | intro (mem : s.rtr[.rcn][i] = some rcn) (triggers : rcn.TriggersOn (s.input i)) 
+  | intro (mem : s.rtr[.rcn][i] = some rcn) (triggers : rcn.TriggersOn (s.input i))
 
 structure NextTag (s : State α) (next : Time.Tag) : Prop where
   mem   : next ∈ s.scheduledTags
   bound : s.tag < next
-  least : ∀ g ∈ s.scheduledTags, (s.tag < g) → (next ≤ g)    
+  least : ∀ g ∈ s.scheduledTags, (s.tag < g) → (next ≤ g)
 
-def Closed (s : State α) : Prop := 
+def Closed (s : State α) : Prop :=
   s.progress = s.rtr[.rcn].ids
 
 def Nontrivial (s : State α) : Prop :=
@@ -69,9 +70,9 @@ structure Terminal (s : State α) : Prop where
   closed  : s.Closed
   no_next : ∀ g, ¬s.NextTag g
 
-protected structure Over (over : α) extends State α where 
+protected structure Over (over : α) extends State α where
   rtr_eq       : rtr = over := by rfl
-  progress_sub : progress ⊆ rtr[.rcn].ids 
+  progress_sub : progress ⊆ rtr[.rcn].ids
   events_sub   : events.ids ⊆ rtr[.act].ids
 
 instance {rtr : α} : CoeOut (State.Over rtr) (State α) where
