ReactorModel/Objects/Reactor/Theorems/Accessible.lean
@@ -17,11 +17,11 @@ theorem obj?_preserved (h : c ≠ cpt ∨ j ≠ i) : (update rtr cpt i v)[c][j] 
 
 theorem obj?_preserved_cpt (h : c ≠ cpt := by exact (nomatch ·)) :
     (update rtr cpt i v)[c][j] = rtr[c][j] :=
-  obj?_preserved $ .inl h
+  obj?_preserved <| .inl h
 
 theorem obj?_preserved_id {c : Component.Valued} (h : j ≠ i) :
     (update rtr cpt i v)[c][j] = rtr[c][j] :=
-  obj?_preserved $ .inr h
+  obj?_preserved <| .inr h
 
 theorem obj?_updated : (update rtr cpt i v)[cpt][i] = (fun _ => v) <$> rtr[cpt][i] :=
   lawful rtr cpt i v |>.obj?_updated
@@ -33,7 +33,7 @@ variable [Finite α]
 -- exactly what happens. When `vs.ids ≠ rtr[cpt].ids`, the values whose id is not in
 -- `rtr[cpt].ids ∩ vs.ids` remain unchanged.
 def set (rtr : α) (cpt : Component.Valued) (vs : ID ⇀ Value) : α :=
-  go rtr cpt vs $ Finite.ids rtr cpt
+  go rtr cpt vs <| Finite.ids rtr cpt
 where
   go (rtr : α) (cpt : Component.Valued) (vs : ID ⇀ Value) : List ID → α
     | [] => rtr
@@ -59,24 +59,24 @@ theorem set.go_preserves {c : Component.Valued} {o vs}
     (ho : rtr[c][i] = some o) (h : c ≠ cpt ∨ i ∉ ids ∨ vs i = none) :
     (set.go rtr cpt vs ids)[c][i] = some o := by
   induction ids generalizing rtr o <;> simp_all [go]; split <;> cases h <;> try cases ‹_ ∨ _›
-  case _ hi _ _ h => exact hi ho $ .inl h
-  case _ hi _ _ h => exact hi ho $ .inr $ .inl h.right
-  case _ hi _ _ h => exact hi ho $ .inr $ .inr h
+  case _ hi _ _ h => exact hi ho <| .inl h
+  case _ hi _ _ h => exact hi ho <| .inr <| .inl h.right
+  case _ hi _ _ h => exact hi ho <| .inr <| .inr h
   case inl hd tl hi _ v _ h =>
     have e := @LawfulUpdatable.equiv _ cpt ‹_› v _ rtr
     have ⟨_, ho'⟩ := Equivalent.obj?_some_iff e |>.mp ⟨_, ho⟩
-    simp [hi ho' $ .inl h]
+    simp [hi ho' <| .inl h]
     injection ho' ▸ ho ▸ obj?_preserved_cpt h
   case inr.inl hd tl hi _ v _ h =>
     have e := @LawfulUpdatable.equiv _ cpt ‹_› v _ rtr
     have ⟨_, ho'⟩ := Equivalent.obj?_some_iff e |>.mp ⟨_, ho⟩
     push_neg at h
-    simp [hi ho' $ .inr $ .inl h.right]
+    simp [hi ho' <| .inr <| .inl h.right]
     injection ho' ▸ ho ▸ obj?_preserved_id h.left
   case inr.inr hd tl hi _ v _ h =>
     have hh : i ≠ hd := by by_contra; simp_all
     have ho' := ho ▸ (@LawfulUpdatable.lawful _ _ rtr cpt hd v).obj?_preserved (c := c) (.inr hh)
-    exact hi ho' (.inr $ .inr h)
+    exact hi ho' (.inr <| .inr h)
 
 omit [Finite α] in
 theorem set.go_updated {cpt : Component.Valued} {o vs}
@@ -90,7 +90,7 @@ theorem set.go_updated {cpt : Component.Valued} {o vs}
     have ⟨_, ho'⟩ := Equivalent.obj?_some_iff e |>.mp ⟨_, ho⟩
     by_cases ht : i ∈ tl
     case pos => exact hi ho' hv ht
-    case neg => simp [set.go_preserves ho' (.inr $ .inl ht), ho' ▸ obj?_updated, ho]
+    case neg => simp [set.go_preserves ho' (.inr <| .inl ht), ho' ▸ obj?_updated, ho]
   case cons.inr hd _ hi ht =>
     simp [go]
     split
@@ -104,8 +104,8 @@ theorem set_updated' : (set rtr cpt vs)[cpt] = fun i => rtr[cpt][i] >>= (vs i |>
   ext1 i
   cases ho : rtr[cpt][i] <;> simp [bind, ho, Option.getD] <;> try split
   · exact Equivalent.obj?_none_iff set_equiv |>.mp ho
-  · exact set.go_updated ho ‹_› $ mem_ids_iff.mpr ⟨_, ho⟩
-  · exact set.go_preserves ho $ .inr $ .inr ‹_›
+  · exact set.go_updated ho ‹_› <| mem_ids_iff.mpr ⟨_, ho⟩
+  · exact set.go_preserves ho <| .inr <| .inr ‹_›
 
 theorem set_updated {cpt : Component.Valued} (h : vs.ids = rtr[cpt].ids) :
     (set rtr cpt vs)[cpt] = vs := by
