ReactorModel/Objects/Reactor/Updatable.lean
@@ -5,25 +5,25 @@ namespace Reactor
 variable [Reactor α]
 
 -- Note: Without ID-uniqueness this can be satisfied by updating exactly one of the occurrences of
---       the target. Since we have a choice of which target we update, this type isn't a `Prop`. 
+--       the target. Since we have a choice of which target we update, this type isn't a `Prop`.
 --       (We need to be able to eliminate into `Type` in `Member.fromLawfulUpdate`).
 inductive LawfulMemUpdate (cpt : Component.Valued) (i : ID) (v : Value) : α → α → Type
-  | final : 
-    (rtr₁ ≃[cpt][i] rtr₂) → (rtr₁{cpt}{i} = some o) → (rtr₂{cpt}{i} = v) → 
+  | final :
+    (rtr₁ ≃[cpt][i] rtr₂) → (rtr₁{cpt}{i} = some o) → (rtr₂{cpt}{i} = v) →
     LawfulMemUpdate cpt i v rtr₁ rtr₂
-  | nested : 
-    (rtr₁ ≃[.rtr][j] rtr₂) → (rtr₁{.rtr}{j} = some n₁) → (rtr₂{.rtr}{j} = some n₂) → 
+  | nested :
+    (rtr₁ ≃[.rtr][j] rtr₂) → (rtr₁{.rtr}{j} = some n₁) → (rtr₂{.rtr}{j} = some n₂) →
     (LawfulMemUpdate cpt i v n₁ n₂) → LawfulMemUpdate cpt i v rtr₁ rtr₂
 
 -- Note: This isn't a `Prop` because of the explanation on `LawfulMemUpdate`.
 inductive LawfulUpdate (cpt : Component.Valued) (i : ID) (v : Value) (rtr₁ rtr₂ : α)
   | update (u : LawfulMemUpdate cpt i v rtr₁ rtr₂)
-  | notMem (h : IsEmpty $ Member cpt i rtr₁) (eq : rtr₁ = rtr₂)
+  | notMem (h : IsEmpty <| Member cpt i rtr₁) (eq : rtr₁ = rtr₂)
 
 class Updatable (α) extends Reactor α where
-  update : α → (cpt : Component.Valued) → ID → Value → α  
-    
-class LawfulUpdatable (α) extends Updatable α where 
-  lawful : ∀ rtr cpt i v, LawfulUpdate cpt i v rtr (update rtr cpt i v)      
+  update : α → (cpt : Component.Valued) → ID → Value → α
+
+class LawfulUpdatable (α) extends Updatable α where
+  lawful : ∀ rtr cpt i v, LawfulUpdate cpt i v rtr (update rtr cpt i v)
 
 end Reactor
