ReactorModel/Execution/Basic.lean
@@ -5,20 +5,20 @@ open Classical Reactor Execution State
 variable [Hierarchical α]
 
 namespace Execution
-namespace Step 
+namespace Step
 
 inductive Apply : Change → State α → State α → Type
-  | inp {rtr} : (LawfulUpdate .inp i v s.rtr rtr) → Apply (.inp i v) s { s with rtr }    
-  | out {rtr} : (LawfulUpdate .out i v s.rtr rtr) → Apply (.out i v) s { s with rtr }    
-  | stv {rtr} : (LawfulUpdate .stv i v s.rtr rtr) → Apply (.stv i v) s { s with rtr }    
+  | inp {rtr} : (LawfulUpdate .inp i v s.rtr rtr) → Apply (.inp i v) s { s with rtr }
+  | out {rtr} : (LawfulUpdate .out i v s.rtr rtr) → Apply (.out i v) s { s with rtr }
+  | stv {rtr} : (LawfulUpdate .stv i v s.rtr rtr) → Apply (.stv i v) s { s with rtr }
   | act : Apply (.act i t v ) s (s.schedule i t v)
   | mut : Apply (.mut _) s s -- Mutations are currently no-ops.
-  
+
 notation s₁:max " -[" c "]→ " s₂:max => Apply c s₁ s₂
 
 inductive Apply.RTC : Reaction.Output → State α → State α → Type
   | refl  : Apply.RTC [] s s
-  | trans : (s₁ -[hd]→ s₂) → (Apply.RTC tl s₂ s₃) → Apply.RTC (hd :: tl) s₁ s₃  
+  | trans : (s₁ -[hd]→ s₂) → (Apply.RTC tl s₂ s₃) → Apply.RTC (hd :: tl) s₁ s₃
 
 notation s₁:max " -[" cs "]→ " s₂:max => Apply.RTC cs s₁ s₂
 
@@ -33,7 +33,7 @@ inductive Exec : State α → State α → Type
 notation s₁:max " ↓ₑ " s₂:max => Exec s₁ s₂
 
 inductive Time : State α → State α → Type
-  | mk : (Closed s) → (NextTag s g) → (Refresh s.rtr ref $ s.actions g) → 
+  | mk : (Closed s) → (NextTag s g) → (Refresh s.rtr ref <| s.actions g) →
          Time s { s with rtr := ref, tag := g, progress := ∅ }
 
 notation s₁:max " ↓ₜ " s₂:max => Time s₁ s₂
