ReactorModel/Execution/Theorems/Grouped/Basic.lean
@@ -12,52 +12,52 @@ structure Grouped [Hierarchical α] (s₁ s₂ : State α) where
   tail  : Grouped.Tail  tl s₂
 
 -- TODO: Most of the case bashing is copied from `Steps.deterministic`. What is the underlying lemma?
-theorem Grouped.deterministic [Proper α] {s s₁ s₂ : State α} 
+theorem Grouped.deterministic [Proper α] {s s₁ s₂ : State α}
     (n : s.Nontrivial) (ht : s₁.tag = s₂.tag) (hp : s₁.progress = s₂.progress) :
     (Grouped s s₁) → (Grouped s s₂) → s₁ = s₂
   | mk (tl := tl₁) steps₁ tail₁, mk (tl := tl₂) steps₂ tail₂ => by
     replace ht : tl₁.tag = tl₂.tag := tail₁.preserves_tag ▸ ht ▸ tail₂.preserves_tag.symm
     induction steps₁ <;> cases steps₂
     case refl.refl => exact tail₁.deterministic hp tail₂
-    case step.step e₁ _ hi _ e₂ e₂' => 
+    case step.step e₁ _ hi _ e₂ e₂' =>
       cases e₁.deterministic e₂
       exact hi (e₁.preserves_nontrivial n) tail₁ e₂' ht
     all_goals cases ‹Step _ _›
-    case refl.step.time e' e   => exact absurd ht $ ne_of_lt $ lt_of_lt_of_le e.tag_lt e'.tag_le
-    case step.refl.time e' _ e => exact absurd ht.symm $ ne_of_lt $ lt_of_lt_of_le e.tag_lt e'.tag_le
+    case refl.step.time e' e   => exact absurd ht <| ne_of_lt <| lt_of_lt_of_le e.tag_lt e'.tag_le
+    case step.refl.time e' _ e => exact absurd ht.symm <| ne_of_lt <| lt_of_lt_of_le e.tag_lt e'.tag_le
     all_goals cases ‹Steps _ _›
     case refl.step.inst.refl e =>
       cases tail₂.closed_to_none e.closed
       cases tail₁
-      case none   => exact absurd hp $ ne_of_ssubset e.progress_ssubset
+      case none   => exact absurd hp <| ne_of_ssubset e.progress_ssubset
       case some f => exact f.deterministic e.exec hp
     case step.refl.inst.refl e _  =>
       cases tail₁.closed_to_none e.closed
       cases tail₂
-      case none   => exact absurd hp.symm $ ne_of_ssubset e.progress_ssubset
+      case none   => exact absurd hp.symm <| ne_of_ssubset e.progress_ssubset
       case some f => exact e.exec.deterministic f hp
     all_goals cases ‹Step _ _›
-    case refl.step.inst.step.time e _ f' f => exact absurd ht $ ne_of_lt $ e.preserves_tag ▸ lt_of_lt_of_le f.tag_lt f'.tag_le
-    case step.refl.inst.step.time e _ f' f => exact absurd ht.symm $ ne_of_lt $ e.preserves_tag ▸ lt_of_lt_of_le f.tag_lt f'.tag_le
+    case refl.step.inst.step.time e _ f' f => exact absurd ht <| ne_of_lt <| e.preserves_tag ▸ lt_of_lt_of_le f.tag_lt f'.tag_le
+    case step.refl.inst.step.time e _ f' f => exact absurd ht.symm <| ne_of_lt <| e.preserves_tag ▸ lt_of_lt_of_le f.tag_lt f'.tag_le
     case refl.step.inst.step.inst e _ f' f => exact e.nonrepeatable f |>.elim
     case step.refl.inst.step.inst e _ f' f => exact e.nonrepeatable f |>.elim
 
-theorem to_grouped [Hierarchical α] {s₁ s₂ : State α} (n : s₁.Nontrivial) (e : s₁ ⇓ s₂) : 
+theorem to_grouped [Hierarchical α] {s₁ s₂ : State α} (n : s₁.Nontrivial) (e : s₁ ⇓ s₂) :
     Nonempty (Grouped s₁ s₂) := by
-  induction e <;> try cases ‹_ ↓ _›  
-  case refl => exact ⟨.refl, .none⟩ 
-  case trans.time hi e => 
-    exact match hi $ e.preserves_nontrivial n with
-    | ⟨.refl, tl⟩              => ⟨.step e .refl, tl⟩ 
-    | ⟨.step (.inst f) f', tl⟩ => ⟨.step (.time e) $ .step f f', tl⟩
+  induction e <;> try cases ‹_ ↓ _›
+  case refl => exact ⟨.refl, .none⟩
+  case trans.time hi e =>
+    exact match hi <| e.preserves_nontrivial n with
+    | ⟨.refl, tl⟩              => ⟨.step e .refl, tl⟩
+    | ⟨.step (.inst f) f', tl⟩ => ⟨.step (.time e) <| .step f f', tl⟩
     | ⟨.step (.time f) _, _⟩   => e.nonrepeatable f n |>.elim
   all_goals
     case _ hi e =>
-      let ⟨steps, tail⟩ := hi $ e.preserves_nontrivial n
+      let ⟨steps, tail⟩ := hi <| e.preserves_nontrivial n
       exact match steps, tail with
-      | .refl,                   .none    => ⟨.refl, .some $ .single e⟩ 
-      | .refl,                   .some e' => ⟨.refl, .some $ .trans e e'⟩
+      | .refl,                   .none    => ⟨.refl, .some <| .single e⟩
+      | .refl,                   .some e' => ⟨.refl, .some <| .trans e e'⟩
       | .step (.inst ⟨f, h⟩) f', tl       => ⟨.step (.inst ⟨.trans e f, h⟩) f', tl⟩
-      | .step (.time f) f',      tl       => ⟨.step (.inst ⟨.single e, f.closed⟩) $ .step f f', tl⟩
+      | .step (.time f) f',      tl       => ⟨.step (.inst ⟨.single e, f.closed⟩) <| .step f f', tl⟩
 
 end Execution
