ReactorModel/Execution/Theorems/Grouped/Steps.lean
@@ -33,9 +33,9 @@ theorem Step.deterministic [Proper α] {s s₁ s₂ : State α} : (Step s s₁) 
   | time e₁, time e₂                    => e₁.deterministic e₂
   | inst e₁, time e₂ | time e₂, inst e₁ => e₁.not_closed e₂.closed |>.elim
 
-inductive Steps [Hierarchical α] : State α → State α → Type 
+inductive Steps [Hierarchical α] : State α → State α → Type
   | refl : Steps s s
-  | step : (Step s₁ s₂) → (Steps s₂ s₃) → Steps s₁ s₃ 
+  | step : (Step s₁ s₂) → (Steps s₂ s₃) → Steps s₁ s₃
 
 namespace Steps
 
@@ -44,22 +44,22 @@ theorem tag_le [Hierarchical α] {s₁ s₂ : State α} (e : Steps s₁ s₂) : 
   case refl => rfl
   case step e _ hi => exact le_trans e.tag_le hi
 
-theorem deterministic [Proper α] {s s₁ s₂ : State α} 
-    (e₁ : Steps s s₁) (e₂ : Steps s s₂) (n : s.Nontrivial) (ht : s₁.tag = s₂.tag) 
+theorem deterministic [Proper α] {s s₁ s₂ : State α}
+    (e₁ : Steps s s₁) (e₂ : Steps s s₂) (n : s.Nontrivial) (ht : s₁.tag = s₂.tag)
     (hp : s₁.progress = s₂.progress) : s₁ = s₂ := by
   induction e₁ <;> cases e₂
   case refl.refl => rfl
-  case step.step e₁ _ hi _ e₂ e₂' => 
+  case step.step e₁ _ hi _ e₂ e₂' =>
     exact hi (e₁.deterministic e₂ ▸ e₂') (e₁.preserves_nontrivial n) ht hp
   all_goals cases ‹Step _ _›
-  case refl.step.time e' e   => exact absurd ht $ ne_of_lt $ lt_of_lt_of_le e.tag_lt e'.tag_le
-  case step.refl.time e' _ e => exact absurd ht.symm $ ne_of_lt $ lt_of_lt_of_le e.tag_lt e'.tag_le
+  case refl.step.time e' e   => exact absurd ht <| ne_of_lt <| lt_of_lt_of_le e.tag_lt e'.tag_le
+  case step.refl.time e' _ e => exact absurd ht.symm <| ne_of_lt <| lt_of_lt_of_le e.tag_lt e'.tag_le
   all_goals cases ‹Steps _ _›
-  case refl.step.inst.refl e' e => exact absurd hp $ ne_of_ssubset e.progress_ssubset
-  case step.refl.inst.refl e _  => exact absurd hp.symm $ ne_of_ssubset e.progress_ssubset
+  case refl.step.inst.refl e' e => exact absurd hp <| ne_of_ssubset e.progress_ssubset
+  case step.refl.inst.refl e _  => exact absurd hp.symm <| ne_of_ssubset e.progress_ssubset
   all_goals cases ‹Step _ _›
-  case refl.step.inst.step.time e _ f' f => exact absurd ht $ ne_of_lt $ e.preserves_tag ▸ lt_of_lt_of_le f.tag_lt f'.tag_le
-  case step.refl.inst.step.time e _ f' f => exact absurd ht.symm $ ne_of_lt $ e.preserves_tag ▸ lt_of_lt_of_le f.tag_lt f'.tag_le
+  case refl.step.inst.step.time e _ f' f => exact absurd ht <| ne_of_lt <| e.preserves_tag ▸ lt_of_lt_of_le f.tag_lt f'.tag_le
+  case step.refl.inst.step.time e _ f' f => exact absurd ht.symm <| ne_of_lt <| e.preserves_tag ▸ lt_of_lt_of_le f.tag_lt f'.tag_le
   case refl.step.inst.step.inst e _ f' f => exact e.nonrepeatable f |>.elim
   case step.refl.inst.step.inst e _ f' f => exact e.nonrepeatable f |>.elim
 
