ReactorModel/Execution/Theorems/Reactor.lean
@@ -5,22 +5,22 @@ namespace Reactor
 
 variable [Hierarchical α]
 
-theorem dependencies_subset (rtr : α) (rcn : ID) : dependencies rtr rcn ⊆ rtr[.rcn].ids := 
+theorem dependencies_subset (rtr : α) (rcn : ID) : dependencies rtr rcn ⊆ rtr[.rcn].ids :=
   fun _ d => d.mem₁
 
-theorem equiv_eq_dependencies {rtr₁ : α} (e : rtr₁ ≈ rtr₂) : 
+theorem equiv_eq_dependencies {rtr₁ : α} (e : rtr₁ ≈ rtr₂) :
   dependencies rtr₁ = dependencies rtr₂ := by
   ext i j
-  exact ⟨.equiv $ .symm e, .equiv e⟩ 
+  exact ⟨.equiv <| .symm e, .equiv e⟩
 
-theorem mem_dependencies_subset {rtr : α} {rcn₁ rcn₂ : ID} (h : rcn₂ ∈ dependencies rtr rcn₁) : 
+theorem mem_dependencies_subset {rtr : α} {rcn₁ rcn₂ : ID} (h : rcn₂ ∈ dependencies rtr rcn₁) :
     dependencies rtr rcn₂ ⊆ dependencies rtr rcn₁ :=
   fun _ h' => Dependency.trans h' h
 
-theorem mem_dependencies_ssubset {rtr : α} {rcn₁ rcn₂ : ID} 
-    (a : Dependency.Acyclic rtr) (h : rcn₂ ∈ dependencies rtr rcn₁) : 
+theorem mem_dependencies_ssubset {rtr : α} {rcn₁ rcn₂ : ID}
+    (a : Dependency.Acyclic rtr) (h : rcn₂ ∈ dependencies rtr rcn₁) :
     dependencies rtr rcn₂ ⊂ dependencies rtr rcn₁ :=
-  ssubset_iff_subset_ne.mpr ⟨mem_dependencies_subset h, (a _ $ ·.symm ▸ h)⟩
+  ssubset_iff_subset_ne.mpr ⟨mem_dependencies_subset h, (a _ <| ·.symm ▸ h)⟩
 
 end Reactor
 
@@ -28,7 +28,7 @@ namespace Reactor
 
 variable [Proper α]
 
-theorem Refresh.deterministic {rtr : α} (rf₁ : Refresh rtr rtr₁ as) (rf₂ : Refresh rtr rtr₂ as) : 
+theorem Refresh.deterministic {rtr : α} (rf₁ : Refresh rtr rtr₁ as) (rf₂ : Refresh rtr rtr₂ as) :
     rtr₁ = rtr₂ := by
   have e := Equivalent.trans (Equivalent.symm rf₁.equiv) rf₂.equiv
   apply ext_obj? e
@@ -41,25 +41,25 @@ theorem Refresh.deterministic {rtr : α} (rf₁ : Refresh rtr rtr₁ as) (rf₂ 
 
 variable [Finite α]
 
-theorem refresh_correct (rtr : α) (h : acts.ids = rtr[.act].ids) : 
+theorem refresh_correct (rtr : α) (h : acts.ids = rtr[.act].ids) :
     Refresh rtr (refresh rtr acts) acts where
-  equiv := Equivalent.trans set_equiv $ Equivalent.trans set_equiv set_equiv
+  equiv := Equivalent.trans set_equiv <| Equivalent.trans set_equiv set_equiv
   eq_state := by
     rw [
-      refresh, set_preserves (by simp : .stv ≠ .act), set_preserves (by simp : .stv ≠ .out), 
+      refresh, set_preserves (by simp : .stv ≠ .act), set_preserves (by simp : .stv ≠ .out),
       set_preserves (by simp : .stv ≠ .inp)
     ]
-  acts := by 
-    rw [refresh, set_updated $ h ▸ (Equivalent.ids_eq $ Equivalent.trans set_equiv set_equiv)]
-  inputs := by 
+  acts := by
+    rw [refresh, set_updated <| h ▸ (Equivalent.ids_eq <| Equivalent.trans set_equiv set_equiv)]
+  inputs := by
     rw [
-      refresh, set_preserves (by simp : .inp ≠ .act), set_preserves (by simp : .inp ≠ .out), 
-      set_updated $ Partial.const_ids _ _, Partial.const_eq_map_const
+      refresh, set_preserves (by simp : .inp ≠ .act), set_preserves (by simp : .inp ≠ .out),
+      set_updated <| Partial.const_ids _ _, Partial.const_eq_map_const
     ]
-  outputs := by 
+  outputs := by
     rw [
       refresh, set_preserves (by simp : .out ≠ .act),
-      set_updated $ by rw [Equivalent.ids_eq set_equiv, Partial.const_ids _ _],
+      set_updated <| by rw [Equivalent.ids_eq set_equiv, Partial.const_ids _ _],
       Partial.const_eq_map_const
     ]
 
