ReactorModel/Execution/Theorems/Trivial.lean
@@ -10,7 +10,7 @@ namespace Execution
 
 variable {s s₁ : State α} in section
 
-abbrev State.Trivial (s : State α) : Prop := 
+abbrev State.Trivial (s : State α) : Prop :=
   s.rtr[.rcn] = ∅
 
 namespace State.Trivial
@@ -28,12 +28,12 @@ namespace Step
 theorem Skip.not_trivial (e : s₁ ↓ₛ s₂) : ¬s₁.Trivial := by
   by_contra ht
   simp [State.Trivial, Partial.empty_iff] at ht
-  cases (Partial.mem_iff.mp e.allows_rcn.mem).choose_spec ▸ ht e.rcn  
+  cases (Partial.mem_iff.mp e.allows_rcn.mem).choose_spec ▸ ht e.rcn
 
 theorem Exec.not_trivial (e : s₁ ↓ₑ s₂) : ¬s₁.Trivial := by
   by_contra ht
   simp [State.Trivial, Partial.empty_iff] at ht
-  cases (Partial.mem_iff.mp e.allows_rcn.mem).choose_spec ▸ ht e.rcn  
+  cases (Partial.mem_iff.mp e.allows_rcn.mem).choose_spec ▸ ht e.rcn
 
 theorem Time.preserves_trivial (triv : s₁.Trivial) (a : s₁ ↓ₜ s₂) : s₂.Trivial :=
   triv.equiv a.equiv
@@ -45,36 +45,36 @@ namespace Step.Time
 
 inductive RTC : State α → State α → Prop
   | refl : RTC s s
-  | trans : (s₁ ↓ₜ s₂) → (RTC s₂ s₃) → RTC s₁ s₃   
+  | trans : (s₁ ↓ₜ s₂) → (RTC s₂ s₃) → RTC s₁ s₃
 
 theorem RTC.tag_le {s₁ s₂ : State α} (e : RTC s₁ s₂) : s₁.tag ≤ s₂.tag := by
   induction e with
   | refl         => exact le_refl _
   | trans a _ hi => exact le_trans (le_of_lt a.tag_lt) hi
 
-theorem RTC.deterministic {s s₁ s₂ : State α} 
+theorem RTC.deterministic {s s₁ s₂ : State α}
     (ht : s₁.tag = s₂.tag) (e₁ : RTC s s₁) (e₂ : RTC s s₂) : s₁ = s₂ := by
   induction e₁ generalizing s₂ <;> cases e₂
   case refl.refl         => rfl
-  case refl.trans e e'   => exact absurd ht      (ne_of_lt $ lt_of_lt_of_le e.tag_lt e'.tag_le)
-  case trans.refl e e' _ => exact absurd ht.symm (ne_of_lt $ lt_of_lt_of_le e.tag_lt e'.tag_le)
+  case refl.trans e e'   => exact absurd ht      (ne_of_lt <| lt_of_lt_of_le e.tag_lt e'.tag_le)
+  case trans.refl e e' _ => exact absurd ht.symm (ne_of_lt <| lt_of_lt_of_le e.tag_lt e'.tag_le)
   case trans.trans e₁ e₁' hi _ e₂ e₂' => exact hi ht (e₂.deterministic e₁ ▸ e₂')
-  
+
 end Step.Time
 
-variable {s s₁ s₂ : State α} 
+variable {s s₁ s₂ : State α}
 
 theorem to_timeStepRTC (triv : s₁.Trivial) (e : s₁ ⇓ s₂) : Step.Time.RTC s₁ s₂ := by
   induction e <;> try cases ‹_ ↓ _›
-  case refl            => exact .refl  
+  case refl            => exact .refl
   case trans.skip e    => exact absurd triv e.not_trivial
   case trans.exec e    => exact absurd triv e.not_trivial
-  case trans.time hi e => exact .trans e (hi $ e.preserves_trivial triv)
+  case trans.time hi e => exact .trans e (hi <| e.preserves_trivial triv)
 
-theorem trivial_deterministic 
+theorem trivial_deterministic
     (triv : ¬s.Nontrivial) (e₁ : s ⇓ s₁) (e₂ : s ⇓ s₂) (ht : s₁.tag = s₂.tag) : s₁ = s₂ :=
   Step.Time.RTC.deterministic ht
-    (e₁.to_timeStepRTC $ .of_not_nontrivial triv) 
-    (e₂.to_timeStepRTC $ .of_not_nontrivial triv) 
+    (e₁.to_timeStepRTC <| .of_not_nontrivial triv)
+    (e₂.to_timeStepRTC <| .of_not_nontrivial triv)
 
 end Execution
