ReactorModel/Objects/Reactor/Finite.lean
@@ -1,3 +1,4 @@
+import Mathlib.Data.Set.Finite.Basic
 import ReactorModel.Objects.Reactor.Hierarchical
 
 noncomputable section
@@ -8,6 +9,6 @@ class Finite (α) [Hierarchical α] where
   fin : ∀ (rtr : α) (cpt : Component), rtr[cpt].Finite
 
 def Finite.ids [Hierarchical α] [Finite α] (rtr : α) (cpt : Component) : List cpt.idType :=
-  (fin rtr cpt).toFinset.toList 
+  (fin rtr cpt).toFinset.toList
 
 namespace Reactor
