ReactorModel/Objects/Reactor/Theorems/Readable.lean
@@ -3,13 +3,13 @@ import ReactorModel.Objects.Reactor.Theorems.Extensional
 
 namespace Reactor
 
-class Readable (α) extends Hierarchical α, Extensional α  
+class Readable (α) extends Hierarchical α, Extensional α
 
 variable [Readable α] {rtr rtr₁ : α}
 
 -- TODO: For simplification of this proof, see comments above `StrictMember.rtr_equiv`.
-theorem LawfulMemUpdate.unique 
-    (u₁ : LawfulMemUpdate cpt i v rtr rtr₁) (u₂ : LawfulMemUpdate cpt i v rtr rtr₂) : 
+theorem LawfulMemUpdate.unique
+    (u₁ : LawfulMemUpdate cpt i v rtr rtr₁) (u₂ : LawfulMemUpdate cpt i v rtr rtr₂) :
     rtr₁ = rtr₂ := by
   induction u₁ generalizing rtr₂ <;> cases u₂
   case final.final e₁ _ h₁' _ _ h₂' e₂ =>
@@ -17,17 +17,17 @@ theorem LawfulMemUpdate.unique
   case nested.nested j₁ _ _ _ _ e₁ h₁ h₁' u₁ hi j₂ _ _ u₂ h₂ h₂' e₂ =>
     have h : j₁ = j₂ := by injection (u₁.member₁.nested h₁).unique (u₂.member₁.nested h₂)
     subst h; cases h₁ ▸ h₂; cases hi u₂
-    exact RootEqualUpTo.ext (RootEqualUpTo.trans e₁.symm e₂) $ h₁' ▸ h₂'.symm
+    exact RootEqualUpTo.ext (RootEqualUpTo.trans e₁.symm e₂) <| h₁' ▸ h₂'.symm
   case final.nested h₁ _ _ _ _ u h₂ _ _ =>
     injection (StrictMember.final h₁).unique (u.member₁.nested h₂)
   case nested.final h₁ _ u _ _ h₂ _ _ =>
     injection (StrictMember.final h₂).unique (u.member₁.nested h₁)
-  
-theorem LawfulUpdate.unique 
+
+theorem LawfulUpdate.unique
     (u₁ : LawfulUpdate cpt i v rtr rtr₁) (u₂ : LawfulUpdate cpt i v rtr rtr₂) : rtr₁ = rtr₂ := by
   cases u₁ <;> cases u₂
   case notMem.notMem => simp_all
   case update.update u₁ u₂ => exact u₁.unique u₂
-  all_goals exact ‹IsEmpty _›.elim $ Member.strict ‹LawfulMemUpdate ..›.member₁
+  all_goals exact ‹IsEmpty _›.elim <| Member.strict ‹LawfulMemUpdate ..›.member₁
 
 end Reactor
